IO.Behavior.fst
@@ -1,0 +1,366 @@
+module IO.Behavior
+
+open FStar.Calc
+open FStar.Tactics
+
+open Common
+open IO.Free
+open IOStHist
+
+type set_of_traces (a:Type) = events_trace * a -> Type0
+
+let empty_set (#a:Type) () : set_of_traces a = fun (t,r) -> t == []
+let pi_to_set #a (pi : check_type) : set_of_traces a = fun (t, _) -> enforced_globally pi (List.rev t)
+
+
+val included_in : (#a:Type) -> (#b:Type) -> (b -> a) -> set_of_traces a -> set_of_traces b -> Type0
+let included_in rel s1 s2 = forall t r1. s1 (t, r1) ==>  (exists r2. rel r2 == r1 /\ s2 (t, r2))
+
+let rec behavior #a
+  (m : io a) : set_of_traces (maybe a) =
+  match m with
+  | Return x -> fun t -> t == ([], Inl x)
+  | Throw err -> fun t -> t == ([], Inr err)
+  | Cont t -> begin
+    match t with
+    | Call cmd args fnc -> (fun (t', r') -> 
+      (exists (res:resm cmd) t. (
+         FStar.WellFounded.axiom1 fnc res;
+         (behavior (fnc res) (t,r')) /\
+         t' == (convert_call_to_event cmd args res)::t)))
+  end
+
+let beh_shift_trace
+  #a
+  (cmd : io_cmds)
+  (argz : args cmd)
+  (rez : resm cmd)
+  (fnc : resm cmd -> io a)
+  (t:events_trace)
+  (r:maybe a) :
+  Lemma 
+    (requires (behavior (Cont (Call cmd argz fnc)) ((convert_call_to_event cmd argz rez :: t), r)))
+    (ensures (behavior (fnc rez) (t, r))) = 
+  () 
+
+let beh_extend_trace 
+  #a
+  (cmd : io_cmds)
+  (argz : args cmd)
+  (rez : resm cmd)
+  (fnc : resm cmd -> io a)
+  (t:events_trace)
+  (r:maybe a) :
+  Lemma
+    (requires (behavior (fnc rez) (t, r)))
+    (ensures (behavior (Cont (Call cmd argz fnc)) ((convert_call_to_event cmd argz rez) :: t, r))) 
+  by (compute ()) = 
+  ()
+
+let beh_extend_trace_d
+  #a
+  (cmd : io_cmds)
+  (argz : args cmd)
+  (rez : resm cmd)
+  (fnc : resm cmd -> io a)
+  (t:events_trace) :
+  Lemma
+    (forall r. (behavior (fnc rez) (t, r) ==>
+      (behavior (Cont (Call cmd argz fnc)) ((convert_call_to_event cmd argz rez) :: t, r)))) =
+  Classical.forall_intro (
+    Classical.move_requires (beh_extend_trace cmd argz rez fnc t))
+
+let beh_extend_trace_in_bind 
+  #a #b
+  (cmd : io_cmds)
+  (argz : args cmd)
+  (rez : resm cmd)
+  (fnc : resm cmd -> io a)
+  (k : a -> io b)
+  (t:events_trace)
+  (r:maybe b) :
+  Lemma
+    (requires (behavior (io_bind a b (fnc rez) k) (t, r))) 
+    (ensures (behavior (io_bind a b (Cont (Call cmd argz fnc)) k) ((convert_call_to_event cmd argz rez) :: t, r))) =
+  calc (==) {
+    io_bind a b (Cont (Call cmd argz fnc)) k;
+    == {}
+    sys_bind io_cmds io_cmd_sig a b (Cont (Call cmd argz fnc)) k;
+    == { _ by (norm [iota; delta]; compute ()) }
+    Cont (sysf_fmap (fun fnci -> 
+      sys_bind io_cmds io_cmd_sig a b fnci k) (Call cmd argz fnc));
+    == { _ by (unfold_def(`sysf_fmap); norm [iota]; unfold_def(`io_bind)) }
+    Cont (Call cmd argz (fun rez -> 
+      io_bind a b (fnc rez) k));
+  };
+  beh_extend_trace cmd argz rez (fun rez -> io_bind a b (fnc rez) k) t r;
+  assert (behavior (Cont (Call cmd argz (fun rez -> 
+    io_bind a b (fnc rez) k))) ((convert_call_to_event cmd argz rez) :: t, r)) by (
+    unfold_def (`convert_call_to_event); assumption ())
+
+let extract_result (cmd:io_cmds) (event:io_event) : 
+  Pure (resm cmd)
+    (requires ((cmd == Openfile /\ EOpenfile? event) \/
+               (cmd == Read /\ ERead? event) \/
+               (cmd == Close /\ EClose? event)))
+    (ensures (fun r -> True)) = 
+  match cmd with 
+  | Openfile -> EOpenfile?.r event 
+  | Read -> ERead?.r event 
+  | Close -> EClose?.r event 
+    
+let rec beh_bind_inl
+  #a #b
+  (m : io a)
+  (k : a -> io b) 
+  (r1:a) 
+  (t1 t2 : events_trace)
+  (r2:maybe b) :
+  Lemma 
+    (requires (behavior m (t1, (Inl r1)) /\ behavior (k r1) (t2, r2)))
+    (ensures (behavior (io_bind _ _ m k) (t1 @ t2, r2))) =
+  match m with
+  | Return x -> ()
+  | Throw err -> ()
+  | Cont (Call cmd argz fnc) -> begin
+    let (ht1 :: tt1) = t1 in
+    let rez : resm cmd = extract_result cmd ht1 in
+    FStar.WellFounded.axiom1 fnc rez;
+    beh_shift_trace cmd argz rez fnc tt1 (Inl r1);
+    beh_bind_inl (fnc rez) k r1 tt1 t2 r2;
+    beh_extend_trace_in_bind cmd argz rez fnc k (tt1@t2) r2
+  end
+  
+let rec beh_bind_inr
+  #a #b
+  (m : io a)
+  (k : a -> io b)
+  (r1:exn)
+  (t1 : events_trace) :
+  Lemma 
+    (requires (behavior m (t1, (Inr r1))))
+    (ensures (behavior (io_bind _ _ m k) (t1, (Inr r1)))) =
+  match m with
+  | Throw err -> ()
+  | Cont (Call cmd argz fnc) -> begin
+    let (ht1 :: tt1) = t1 in
+    let rez : resm cmd = extract_result cmd ht1 in
+    FStar.WellFounded.axiom1 fnc rez;
+    beh_shift_trace cmd argz rez fnc tt1 (Inr r1);
+    beh_bind_inr (fnc rez) k r1 tt1;
+    beh_extend_trace_in_bind cmd argz rez fnc k (tt1) (Inr r1)
+  end
+
+let beh_bind_0 
+  #a #b
+  (m : io a)
+  (k : a -> io b) 
+  (r1:maybe a) :
+  Lemma (forall t1.
+    behavior m (t1, r1) ==>
+      (Inr? r1 ==>  behavior (io_bind _ _ m k) (t1, (Inr (Inr?.v r1)))) /\
+      (Inl? r1 ==>  (forall t2 r2. (behavior (k (Inl?.v r1)) (t2, r2) ==>  
+                     behavior (io_bind _ _ m k) (t1 @ t2, r2))))) =
+  if (Inr? r1) then (
+    Classical.forall_intro (
+      Classical.move_requires (beh_bind_inr m k (Inr?.v r1)))
+  ) else (
+    Classical.forall_intro_3 (
+      Classical.move_requires_3 (beh_bind_inl m k (Inl?.v r1)))
+  )
+
+let beh_bind
+  #a #b
+  (m : io a)
+  (k : a -> io b) :
+  Lemma (forall (r1:maybe a) t1.
+    behavior m (t1, r1) ==>
+      (Inr? r1 ==>  behavior (io_bind _ _ m k) (t1, (Inr (Inr?.v r1)))) /\
+      (Inl? r1 ==>  (forall t2 r2. behavior (k (Inl?.v r1)) (t2, r2) ==>  
+                              behavior (io_bind _ _ m k) (t1 @ t2, r2)))) =
+  Classical.forall_intro (beh_bind_0 m k)
+
+let rec beh_bind_tot_0
+  #a #b
+  (f:io a) 
+  (g:a -> Tot b)
+  (r1:maybe b)
+  (t:events_trace) :
+  Lemma 
+    (requires (behavior (io_bind a b f (fun x -> M4.lift_pure_m4wp b (fun p -> p (g x)) (fun _ -> g x) (fun _ -> True))) (t, r1)))
+    (ensures (exists r2. inl_app g r2 == r1 /\ behavior f (t, r2)))  =
+  match f with
+  | Return x -> 
+      assert (inl_app g (Inl x) == r1);
+      assert (behavior f (t, (Inl x)))
+  | Throw err -> 
+      assert (inl_app g (Inr err) == r1);
+      assert (behavior f (t, (Inr err)))
+  | Cont (Call cmd argz fnc) ->
+    let (ht1 :: tt1) = t in
+    let rez : resm cmd = extract_result cmd ht1 in
+    FStar.WellFounded.axiom1 fnc rez;
+    beh_bind_tot_0 (fnc rez) g r1 tt1;
+    beh_extend_trace_d cmd argz rez fnc (tt1)
+       
+let beh_bind_tot
+  #a #b
+  (f:io a)
+  (g:a -> Tot b) :
+  Lemma 
+    (forall r1 t. (behavior (io_bind a b f (fun x -> M4.lift_pure_m4wp b (fun p -> p (g x)) (fun _ -> g x) (fun _ -> True))) (t, r1)) ==>  (exists r2. r1 == inl_app g r2 /\ behavior f (t,r2))) =
+  Classical.forall_intro_2 (Classical.move_requires_2 (beh_bind_tot_0 f g))
+
+let beh_included_bind_tot
+  #a #b
+  (f:io a) 
+  (g:a -> Tot b) :
+  Lemma
+    (included_in (inl_app g)
+      (behavior (io_bind a b f (fun x -> M4.lift_pure_m4wp b (fun p -> p (g x)) (fun _ -> g x) (fun _ -> True))))
+      (behavior f)) = 
+  beh_bind_tot f g
+
+let beh_iost_to_io (a:Type) (tree:io (events_trace * a)) :
+  Lemma (behavior (IOStHist.iost_to_io tree) `included_in (inl_app cdr)` behavior tree) 
+  by (unfold_def (`IOStHist.iost_to_io); norm [iota;delta]; compute ()) =
+  beh_included_bind_tot #(events_trace * a) #a
+    tree
+    cdr
+
+unfold let ref #a (x : io a) : M4.irepr a (fun p -> forall res. p res) = (fun _ -> x)
+
+let beh_included_in_trans_id x y z :
+  Lemma (
+    (behavior x `included_in id` behavior y /\
+    behavior y `included_in id` behavior z) ==>
+      behavior x `included_in id` behavior z) = ()
+  
+let beh_included_in_trans_id_g x y z g:
+  Lemma (
+    (behavior x `included_in id` behavior y /\
+    behavior y `included_in g` behavior z) ==>
+      behavior x `included_in g` behavior z) = ()
+  
+let beh_included_in_trans_g_id x y z g:
+  Lemma (
+    (behavior x `included_in g` behavior y /\
+    behavior y `included_in id` behavior z) ==>
+      behavior x `included_in g` behavior z) = ()
+
+let beh_included_in_merge_f_g x y z f g:
+  Lemma (
+    (behavior x `included_in f` behavior y /\
+    behavior y `included_in g` behavior z) ==>
+      behavior x `included_in (compose f g)` behavior z) = ()
+
+
+let rec beh_implies_iohist_interp 
+  (a : Type)
+  (m : io (events_trace * a)) 
+  (h : events_trace)
+  (t : events_trace)
+  (r : maybe (events_trace * a)) :
+  Lemma 
+    (requires (behavior m (t,r)))
+    (ensures (iohist_interpretation m h (fun res le -> (t,res) == (le,r)))) = 
+  match m with
+  | Return _ -> ()
+  | Throw _ -> ()
+  | Cont (Call cmd argz fnc) -> admit ()
+
+let gio_post_implies_set_of_traces 
+  (a : Type)
+  (b : Type)
+  (pi : check_type)
+  (t : events_trace)
+  (r : maybe (events_trace * b)) :
+  Lemma 
+    (requires  (gio_post pi [] r t))
+    (ensures (pi_to_set pi (t, r))) = 
+    List.Tot.Properties.append_l_nil (List.rev t);
+    ()
+
+let iohist_interp_shift_trace
+  #a
+  (cmd : io_cmds)
+  (argz : args cmd)
+  (rez : resm cmd)
+  (fnc : resm cmd -> io a)
+  (h:events_trace)
+  p:
+  Lemma 
+    (requires (iohist_interpretation (Cont (Call cmd argz fnc)) h p))
+    (ensures (
+      iohist_interpretation (fnc rez) (convert_call_to_event cmd argz rez :: h) (gen_post p (convert_call_to_event cmd argz rez)))) = 
+  calc (==) {
+    iohist_interpretation (Cont (Call cmd argz fnc)) h p;
+    == { _ by (compute ())}
+    (forall res. (
+      let event : io_event = convert_call_to_event cmd argz res in
+      iohist_interpretation (fnc res) (event :: h) (gen_post p event)));
+  }
+
+let rec gio_interpretation_implies_set_of_traces
+  (a : Type)
+  (pi : check_type)
+  (m : io (events_trace * a)) 
+  (h : events_trace)
+  (le : events_trace)
+  (r : maybe (events_trace * a)) 
+  p :
+  Lemma 
+    (requires (iohist_interpretation m h p) /\ behavior m (le, r))
+    (ensures (p r le)) =
+  match m with
+  | Return _ -> ()
+  | Throw _ -> ()
+  | Cont (Call cmd argz fnc) -> begin
+    let (ht1 :: tt1) = le in
+    let rez : resm cmd = extract_result cmd ht1 in
+    FStar.WellFounded.axiom1 fnc rez;
+    beh_shift_trace cmd argz rez fnc tt1 r;
+    iohist_interp_shift_trace cmd argz rez fnc h p;
+    gio_interpretation_implies_set_of_traces a pi (fnc rez) (convert_call_to_event cmd argz rez :: h) tt1 r (gen_post p (convert_call_to_event cmd argz rez))
+  end
+
+
+unfold 
+let beh #a #b (pi:check_type) (ws:a -> GIO b pi) (x:a) =
+  behavior (reify (ws x) (gio_post pi []) [])
+  
+let beh_gio_implies_post 
+  (a : Type)
+  (b : Type)
+  (pi : check_type)
+  (ws : a -> GIO b pi) 
+  (x : a)
+  (t : events_trace)
+  (r : maybe (events_trace * b)) :
+  Lemma 
+    (requires (beh pi ws x (t, r)))
+    (ensures  (gio_post pi [] r t)) =
+  let ws' = reify (ws x) (gio_post pi []) [] in
+  gio_interpretation_implies_set_of_traces b pi ws' [] t r (gio_post pi []) 
+
+let beh_gio_in_pi_0 
+  (a b : Type)
+  (pi : check_type)
+  (ws : a -> GIO b pi) 
+  (x : a)
+  (t : events_trace)
+  (r : maybe (events_trace * b)) :
+  Lemma 
+    (requires ((beh pi ws x) (t, r)))
+    (ensures  ((pi_to_set pi) (t, r))) =
+  beh_gio_implies_post a b pi ws x t r;
+  gio_post_implies_set_of_traces a b pi t r
+  
+let beh_gio_in_pi
+  (a b : Type)
+  (pi : check_type)
+  (ws : a -> GIO b pi) 
+  (x : a) :
+  Lemma (beh pi ws x `included_in id` pi_to_set pi) =
+  Classical.forall_intro_2 (Classical.move_requires_2 (beh_gio_in_pi_0 a b pi ws x))
+  
